packages/zoe/spec/jessie_justin.v
@@ -1,4 +1,4 @@
-From Coq Require Import Bool List String ZArith.
+From Coq Require Import Bool Lia List String ZArith.
 Require Import jessie_lang.
 
 Import ListNotations.
@@ -241,6 +241,29 @@ Module JustinExec.
     in
     (VLoc obj, σ').
 
+  Definition alloc_counter_cap (σ : state) (counter : val) (field : string)
+    : option (val * state) :=
+    match counter with
+    | VLoc l =>
+        match lookup_obj σ l with
+        | Some obj =>
+            match lookup_field (obj_fields obj) field with
+            | Some method =>
+                let '(cap, σ1) := alloc_obj σ [(field, method)] in
+                Some (cap, freeze_deep 20 σ1 cap)
+            | None => None
+            end
+        | None => None
+        end
+    | _ => None
+    end.
+
+  Definition alloc_entry_cap (σ : state) (counter : val) : option (val * state) :=
+    alloc_counter_cap σ counter "incr".
+
+  Definition alloc_exit_cap (σ : state) (counter : val) : option (val * state) :=
+    alloc_counter_cap σ counter "decr".
+
   Definition apply_prim (σ : state) (name : string) (args : list val)
     : core_expr * state :=
     if String.eqb name "makeCounter" then
@@ -296,6 +319,198 @@ Module JustinExec.
           end
       | None => (CoreBzzt, σ)
       end.
+
+  Definition invoke_cap_method (σ : state) (cap : val) (field : string)
+    : option (val * state) :=
+    match cap with
+    | VLoc l =>
+        match lookup_obj σ l with
+        | Some obj =>
+            match lookup_field (obj_fields obj) field with
+            | Some (VPrim name) =>
+                match apply_prim σ name [] with
+                | (CoreLit v, σ') => Some (v, σ')
+                | _ => None
+                end
+            | _ => None
+            end
+        | None => None
+        end
+    | _ => None
+    end.
+
+  Fixpoint invoke_cap_trace (σ : state) (cap : val) (trace : list string)
+    : option state :=
+    match trace with
+    | [] => Some σ
+    | field :: trace' =>
+        match invoke_cap_method σ cap field with
+        | Some (_, σ') => invoke_cap_trace σ' cap trace'
+        | None => None
+        end
+    end.
+
+  Lemma lookup_obj_store_cell σ cell n l :
+    lookup_obj (store_cell σ cell n) l = lookup_obj σ l.
+  Proof. reflexivity. Qed.
+
+  Lemma lookup_dyn_store_cell σ cell n name :
+    lookup_assoc name (st_dyn_prims (store_cell σ cell n)) =
+      lookup_assoc name (st_dyn_prims σ).
+  Proof. reflexivity. Qed.
+
+  Lemma store_cell_list_overwrite cells l n1 n2 :
+    store_cell_list (store_cell_list cells l n1) l n2 =
+      store_cell_list cells l n2.
+  Proof.
+    induction cells as [|[l' n'] cells IH]; simpl.
+    - now rewrite Nat.eqb_refl.
+    - destruct (Nat.eqb l l') eqn:Heq.
+      + apply Nat.eqb_eq in Heq. subst. simpl. now rewrite Nat.eqb_refl.
+      + simpl. rewrite Heq. f_equal. exact IH.
+  Qed.
+
+  Lemma store_cell_overwrite σ cell n1 n2 :
+    store_cell (store_cell σ cell n1) cell n2 = store_cell σ cell n2.
+  Proof.
+    destruct σ as [next store frozen env cells dyn].
+    unfold store_cell. simpl.
+    rewrite store_cell_list_overwrite.
+    reflexivity.
+  Qed.
+
+  Lemma lookup_cell_store_same σ cell n :
+    lookup_cell (store_cell σ cell n) cell = Some n.
+  Proof.
+    unfold lookup_cell, store_cell.
+    simpl.
+    induction (st_cells σ) as [|[l' n'] cells IH]; simpl.
+    - now rewrite Nat.eqb_refl.
+    - destruct (Nat.eqb cell l') eqn:Heq.
+      + apply Nat.eqb_eq in Heq. subst. simpl. now rewrite Nat.eqb_refl.
+      + simpl. rewrite Heq. exact IH.
+  Qed.
+
+  Lemma store_cell_list_same cells l n :
+    lookup_cell_list cells l = Some n ->
+    store_cell_list cells l n = cells.
+  Proof.
+    induction cells as [|[l' n'] cells IH]; simpl; [discriminate|].
+    destruct (Nat.eqb l l') eqn:Heq.
+    - apply Nat.eqb_eq in Heq. subst.
+      intros [= <-]. simpl. reflexivity.
+    - intros Hlookup. simpl. f_equal. apply IH. exact Hlookup.
+  Qed.
+
+  Lemma store_cell_same_value σ cell n :
+    lookup_cell σ cell = Some n ->
+    store_cell σ cell n = σ.
+  Proof.
+    destruct σ as [next store frozen env cells dyn].
+    unfold store_cell, lookup_cell. simpl.
+    intros Hlookup. f_equal.
+    apply store_cell_list_same. exact Hlookup.
+  Qed.
+
+  Lemma invoke_entry_cap_step σ capl cell n :
+    lookup_obj σ capl =
+      Some (HeapObj [("incr", VPrim (counter_incr_name cell))]) ->
+    lookup_assoc (counter_incr_name cell) (st_dyn_prims σ) =
+      Some (CounterIncr cell) ->
+    lookup_cell σ cell = Some n ->
+    invoke_cap_method σ (VLoc capl) "incr" =
+      Some (VJson (JNum (n + 1)), store_cell σ cell (n + 1)).
+  Proof.
+    intros Hobj Hdyn Hcell.
+    unfold invoke_cap_method.
+    rewrite Hobj. simpl.
+    unfold apply_prim.
+    assert (Hmk : counter_incr_name cell <> "makeCounter"). { discriminate. }
+    assert (Has : counter_incr_name cell <> "assert"). { discriminate. }
+    assert (Hid : counter_incr_name cell <> "id"). { discriminate. }
+    assert (Hfail : counter_incr_name cell <> "fail"). { discriminate. }
+    assert (Hfreeze : counter_incr_name cell <> "freeze"). { discriminate. }
+    assert (Hharden : counter_incr_name cell <> "harden"). { discriminate. }
+    pose proof ((proj2 (String.eqb_neq _ _)) Hmk) as Hmkb.
+    pose proof ((proj2 (String.eqb_neq _ _)) Has) as Hasb.
+    pose proof ((proj2 (String.eqb_neq _ _)) Hid) as Hidb.
+    pose proof ((proj2 (String.eqb_neq _ _)) Hfail) as Hfailb.
+    pose proof ((proj2 (String.eqb_neq _ _)) Hfreeze) as Hfreezeb.
+    pose proof ((proj2 (String.eqb_neq _ _)) Hharden) as Hhardenb.
+    rewrite Hmkb.
+    rewrite Hasb.
+    rewrite Hidb.
+    rewrite Hfailb.
+    rewrite Hfreezeb.
+    rewrite Hhardenb.
+    rewrite Hdyn.
+    rewrite Hcell.
+    reflexivity.
+  Qed.
+
+  Lemma invoke_exit_cap_step σ capl cell n :
+    lookup_obj σ capl =
+      Some (HeapObj [("decr", VPrim (counter_decr_name cell))]) ->
+    lookup_assoc (counter_decr_name cell) (st_dyn_prims σ) =
+      Some (CounterDecr cell) ->
+    lookup_cell σ cell = Some n ->
+    invoke_cap_method σ (VLoc capl) "decr" =
+      Some (VJson (JNum (n - 1)), store_cell σ cell (n - 1)).
+  Proof.
+    intros Hobj Hdyn Hcell.
+    unfold invoke_cap_method.
+    rewrite Hobj. simpl.
+    unfold apply_prim.
+    assert (Hmk : counter_decr_name cell <> "makeCounter"). { discriminate. }
+    assert (Has : counter_decr_name cell <> "assert"). { discriminate. }
+    assert (Hid : counter_decr_name cell <> "id"). { discriminate. }
+    assert (Hfail : counter_decr_name cell <> "fail"). { discriminate. }
+    assert (Hfreeze : counter_decr_name cell <> "freeze"). { discriminate. }
+    assert (Hharden : counter_decr_name cell <> "harden"). { discriminate. }
+    pose proof ((proj2 (String.eqb_neq _ _)) Hmk) as Hmkb.
+    pose proof ((proj2 (String.eqb_neq _ _)) Has) as Hasb.
+    pose proof ((proj2 (String.eqb_neq _ _)) Hid) as Hidb.
+    pose proof ((proj2 (String.eqb_neq _ _)) Hfail) as Hfailb.
+    pose proof ((proj2 (String.eqb_neq _ _)) Hfreeze) as Hfreezeb.
+    pose proof ((proj2 (String.eqb_neq _ _)) Hharden) as Hhardenb.
+    rewrite Hmkb.
+    rewrite Hasb.
+    rewrite Hidb.
+    rewrite Hfailb.
+    rewrite Hfreezeb.
+    rewrite Hhardenb.
+    rewrite Hdyn.
+    rewrite Hcell.
+    reflexivity.
+  Qed.
+
+  Lemma invoke_entry_cap_other_none σ capl cell field :
+    lookup_obj σ capl =
+      Some (HeapObj [("incr", VPrim (counter_incr_name cell))]) ->
+    field <> "incr" ->
+    invoke_cap_method σ (VLoc capl) field = None.
+  Proof.
+    intros Hobj Hneq.
+    unfold invoke_cap_method.
+    rewrite Hobj. simpl.
+    destruct (String.eqb field "incr") eqn:Heq.
+    - apply String.eqb_eq in Heq. subst field. contradiction.
+    - reflexivity.
+  Qed.
+
+  Lemma invoke_exit_cap_other_none σ capl cell field :
+    lookup_obj σ capl =
+      Some (HeapObj [("decr", VPrim (counter_decr_name cell))]) ->
+    field <> "decr" ->
+    invoke_cap_method σ (VLoc capl) field = None.
+  Proof.
+    intros Hobj Hneq.
+    unfold invoke_cap_method.
+    rewrite Hobj. simpl.
+    destruct (String.eqb field "decr") eqn:Heq.
+    - apply String.eqb_eq in Heq. subst field. contradiction.
+    - reflexivity.
+  Qed.
 
   Fixpoint step (σ : state) (e : core_expr) : option (core_expr * state) :=
     match e with
